Stuck on big boy proofs

language_formalisation/type_system/type_aux_lemmas.v
@@ -6,141 +6,155 @@ Add LoadPath "C:\Users\Ziga\Documents\Ziga_podatki\PHD\language_formalisation\su
 (* Add LoadPath "E:\Ziga_Podatki\faks\PHD\language_formalisation\substitution". *)
 
 Require Export syntax syntax_lemmas declarational substitution Omega Logic.
-Require Export subs_lemmas wellfounded_lemmas.
+Require Export subs_lemmas subtyping wellfounded_lemmas.
 
 Ltac inv H := inversion H; clear H; subst.
 
 
-Fixpoint v_insert_typesafe v Γ A A_ins i {struct v} :
-  has_vtype Γ v A -> wf_vtype A_ins ->
+Fixpoint v_insert_typesafe 
+  Γ v A (orig : has_vtype Γ v A) A_ins i {struct orig} :
+  wf_vtype A_ins ->
   has_vtype (ctx_insert_var Γ A_ins i) (Sub.v_shift v 1 i) A
-with c_insert_typesafe c Γ C A_ins i {struct c} :
-  has_ctype Γ c C -> wf_vtype A_ins ->
+
+with c_insert_typesafe 
+  Γ c C (orig : has_ctype Γ c C) A_ins i {struct orig} :
+  wf_vtype A_ins ->
   has_ctype (ctx_insert_var Γ A_ins i) (Sub.c_shift c 1 i) C
-with h_insert_typesafe h Γ Σ D A_ins i {struct h} :
-  has_htype Γ h Σ D -> wf_vtype A_ins ->
+
+with h_insert_typesafe 
+  Γ h Σ D (orig : has_htype Γ h Σ D) A_ins i {struct orig} :
+  wf_vtype A_ins ->
   has_htype (ctx_insert_var Γ A_ins i) (Sub.h_shift h 1 i) Σ D.
 Proof.
 {
-intros orig wfins. apply TypeV.
-{ clear v_insert_typesafe c_insert_typesafe h_insert_typesafe.
-  apply ctx_insert_wf. inv orig. assumption. assumption. }
-{ clear v_insert_typesafe c_insert_typesafe h_insert_typesafe.
-  inv orig. assumption. }
-inv orig. destruct v.
+intros wfins. apply TypeV.
+{ apply ctx_insert_wf. inv orig. assumption. assumption. }
+{ inv orig. assumption. }
+inv orig. destruct H1.
 + clear v_insert_typesafe c_insert_typesafe h_insert_typesafe.
-  inv H1. simpl. destruct (i <=? num) eqn:cmp.
+  simpl. apply TypeUnit.
++ clear v_insert_typesafe c_insert_typesafe h_insert_typesafe.
+  simpl. apply TypeInt.
++ clear v_insert_typesafe c_insert_typesafe h_insert_typesafe.
+  simpl. destruct (i <=? num) eqn:cmp.
   - apply TypeVar. rewrite <-get_ctx_insert_changed.
     assumption. apply leb_complete in cmp. omega.
   - apply TypeVar. rewrite <-get_ctx_insert_unchanged.
     assumption. apply leb_iff_conv in cmp. assumption.
-+ clear v_insert_typesafe c_insert_typesafe h_insert_typesafe.
-  inv H1. simpl. apply TypeUnit.
-+ clear v_insert_typesafe c_insert_typesafe h_insert_typesafe.
-  inv H1. simpl. apply TypeInt.
-+ specialize (v_insert_typesafe v) as IHv.
++ specialize (v_insert_typesafe _ _ _ H1) as IHv1.
+  specialize (v_insert_typesafe _ _ _ H2) as IHv2.
   clear v_insert_typesafe c_insert_typesafe h_insert_typesafe.
-  inv H1. simpl. apply TypeInl. apply IHv; assumption.
-+ specialize (v_insert_typesafe v) as IHv.
-  clear v_insert_typesafe c_insert_typesafe h_insert_typesafe.
-  inv H1. simpl. apply TypeInr. apply IHv; assumption.
-+ specialize (v_insert_typesafe v1) as IHv1.
-  specialize (v_insert_typesafe v2) as IHv2.
-  clear v_insert_typesafe c_insert_typesafe h_insert_typesafe.
-  inv H1. simpl. apply TypePair. 
+  simpl. apply TypePair. 
   - apply IHv1; assumption.
   - apply IHv2; assumption.
-+ specialize (c_insert_typesafe c) as IHc.
++ specialize (v_insert_typesafe _ _ _ H1) as IHv.
   clear v_insert_typesafe c_insert_typesafe h_insert_typesafe.
-  inv H1. simpl. apply TypeFun. rewrite ctx_insert_extend.
+  simpl. apply TypeInl. apply IHv; assumption.
++ specialize (v_insert_typesafe _ _ _ H1) as IHv.
+  clear v_insert_typesafe c_insert_typesafe h_insert_typesafe.
+  simpl. apply TypeInr. apply IHv; assumption.
++ specialize (c_insert_typesafe _ _ _ H1) as IHc.
+  clear v_insert_typesafe c_insert_typesafe h_insert_typesafe.
+  simpl. apply TypeFun. rewrite ctx_insert_extend.
   apply IHc; assumption.
-+ specialize (h_insert_typesafe h) as IHh.
-  specialize (c_insert_typesafe c) as IHc.
++ specialize (h_insert_typesafe _ _ _ _ H2) as IHh.
+  specialize (c_insert_typesafe _ _ _ H1) as IHc.
   clear v_insert_typesafe c_insert_typesafe h_insert_typesafe.
-  inv H1. simpl. apply TypeHandler. rewrite ctx_insert_extend. 
+  simpl. apply TypeHandler. rewrite ctx_insert_extend. 
   - apply IHc; assumption. 
   - apply IHh; assumption.
++ specialize (v_insert_typesafe _ _ _ H1) as IHv.
+  clear v_insert_typesafe c_insert_typesafe h_insert_typesafe.
+  eapply TypeVSubtype.
+  - apply IHv. assumption.
+  - assumption.
 }{
-intros orig wfins. apply TypeC.
+intros wfins. apply TypeC.
 { clear v_insert_typesafe c_insert_typesafe h_insert_typesafe.
   apply ctx_insert_wf. inv orig. assumption. assumption. }
 { clear v_insert_typesafe c_insert_typesafe h_insert_typesafe.
   inv orig. assumption. }
-inv orig. destruct c.
-+ specialize (v_insert_typesafe v) as IHv.
+inv orig. destruct H1.
++ specialize (v_insert_typesafe _ _ _ H1) as IHv.
   clear v_insert_typesafe c_insert_typesafe h_insert_typesafe.
-  inv H1. simpl. apply TypeRet. apply IHv; assumption.
-+ specialize (v_insert_typesafe v) as IHv.
-  specialize (c_insert_typesafe c) as IHc.
+  simpl. apply TypeRet. apply IHv; assumption.
++ specialize (v_insert_typesafe _ _ _ H1) as IHv.
+  specialize (c_insert_typesafe _ _ _ H2) as IHc.
   clear v_insert_typesafe c_insert_typesafe h_insert_typesafe.
-  inv H1; simpl. eapply TypeΠMatch.
-  apply IHv. exact H7. assumption.
+  eapply TypeΠMatch.
+  apply IHv. assumption.
   rewrite ctx_insert_extend. rewrite ctx_insert_extend.
-  assert (i+1+1=i+2) by omega. rewrite H1. apply IHc; assumption.
-+ specialize (v_insert_typesafe v) as IHv.
-  specialize (c_insert_typesafe c1) as IHc1.
-  specialize (c_insert_typesafe c2) as IHc2.
+  assert (i+1+1=i+2) by omega. rewrite H3. apply IHc; assumption.
++ specialize (v_insert_typesafe _ _ _ H1) as IHv.
+  specialize (c_insert_typesafe _ _ _ H2) as IHc1.
+  specialize (c_insert_typesafe _ _ _ H3) as IHc2.
   clear v_insert_typesafe c_insert_typesafe h_insert_typesafe.
-  inv H1. simpl. eapply TypeΣMatch.
-  - apply IHv. exact H9. assumption.
+  simpl. eapply TypeΣMatch.
+  - apply IHv. assumption.
   - rewrite ctx_insert_extend. apply IHc1; assumption. 
   - rewrite ctx_insert_extend. apply IHc2; assumption. 
-+ specialize (v_insert_typesafe v) as IHv.
-  specialize (v_insert_typesafe v0) as IHv0.
++ specialize (c_insert_typesafe _ _ _ H1) as IHc1.
+  specialize (c_insert_typesafe _ _ _ H2) as IHc2.
   clear v_insert_typesafe c_insert_typesafe h_insert_typesafe.
-  inv H1. simpl. eapply TypeApp.
-  - apply IHv. exact H5. assumption.
+  simpl. eapply TypeDoBind.
+  - apply IHc1. assumption.
+  - rewrite ctx_insert_extend. apply IHc2; assumption.
++ specialize (v_insert_typesafe _ _ _ H1) as IHv.
+  specialize (v_insert_typesafe _ _ _ H2) as IHv0.
+  clear v_insert_typesafe c_insert_typesafe h_insert_typesafe.
+  simpl. eapply TypeApp.
+  - apply IHv. assumption.
   - apply IHv0; assumption.
-+ specialize (v_insert_typesafe v) as IHv.
-  specialize (c_insert_typesafe c) as IHc.
++ specialize (v_insert_typesafe _ _ _ H1) as IHv.
+  specialize (c_insert_typesafe _ _ _ H2) as IHc.
   clear v_insert_typesafe c_insert_typesafe h_insert_typesafe.
-  inv H1. simpl. eapply TypeOp. exact H8.
+  simpl. eapply TypeHandle.
+  - apply IHv. assumption.
+  - apply IHc; assumption.
++ specialize (c_insert_typesafe _ _ _ H1) as IHc1.
+  specialize (c_insert_typesafe _ _ _ H2) as IHc2.
+  clear v_insert_typesafe c_insert_typesafe h_insert_typesafe.
+  simpl. eapply TypeLetRec.
+  - rewrite ctx_insert_extend. rewrite ctx_insert_extend.
+    assert (i+1+1=i+2) by omega. rewrite H3. apply IHc1. assumption.
+  - rewrite ctx_insert_extend.  apply IHc2; assumption.
++ specialize (v_insert_typesafe _ _ _ H2) as IHv.
+  specialize (c_insert_typesafe _ _ _ H3) as IHc.
+  clear v_insert_typesafe c_insert_typesafe h_insert_typesafe.
+  simpl. eapply TypeOp.
+  - exact H1.
   - apply IHv; assumption.
   - rewrite ctx_insert_extend. apply IHc; assumption.
-+ specialize (c_insert_typesafe c1) as IHc1.
-  specialize (c_insert_typesafe c2) as IHc2.
++ specialize (c_insert_typesafe _ _ _ H1) as IHc.
   clear v_insert_typesafe c_insert_typesafe h_insert_typesafe.
-  inv H1. simpl. eapply TypeLetRec.
-  - rewrite ctx_insert_extend. rewrite ctx_insert_extend.
-    assert (i+1+1=i+2) by omega. rewrite H1. apply IHc1. exact H8. assumption.
-  - rewrite ctx_insert_extend.  apply IHc2; assumption.
-+ specialize (c_insert_typesafe c1) as IHc1.
-  specialize (c_insert_typesafe c2) as IHc2.
-  clear v_insert_typesafe c_insert_typesafe h_insert_typesafe.
-  inv H1. simpl. eapply TypeDoBind.
-  - apply IHc1. exact H7. assumption.
-  - rewrite ctx_insert_extend. apply IHc2; assumption.
-+ specialize (v_insert_typesafe v) as IHv.
-  specialize (c_insert_typesafe c) as IHc.
-  clear v_insert_typesafe c_insert_typesafe h_insert_typesafe.
-  inv H1. simpl. eapply TypeHandle.
-  - apply IHv. exact H5. assumption.
-  - apply IHc; assumption.
+  eapply TypeCSubtype.
+  - apply IHc. assumption.
+  - assumption.
 }{
-intros orig wfins. apply TypeH.
+intros wfins. apply TypeH.
 { clear v_insert_typesafe c_insert_typesafe h_insert_typesafe.
   apply ctx_insert_wf. inv orig. assumption. assumption. }
 { clear v_insert_typesafe c_insert_typesafe h_insert_typesafe.
   inv orig. assumption. }
 { clear v_insert_typesafe c_insert_typesafe h_insert_typesafe.
   inv orig. assumption. }
-inv orig. destruct h.
-+ inv H2. simpl. clear v_insert_typesafe c_insert_typesafe h_insert_typesafe.
+inv orig. destruct H2.
++ simpl. clear v_insert_typesafe c_insert_typesafe h_insert_typesafe.
   apply TypeCasesØ.
-+ specialize (h_insert_typesafe h) as IHh.
-  specialize (c_insert_typesafe c) as IHc.
++ specialize (h_insert_typesafe _ _ _ _ H3) as IHh.
+  specialize (c_insert_typesafe _ _ _ H4) as IHc.
   clear v_insert_typesafe c_insert_typesafe h_insert_typesafe.
-  inv H2. simpl. apply TypeCasesU.
-  - assert (forall h,
-      find_op_case h o = None ->
-      find_op_case (Sub.h_shift h 1 i) o = None).
-    * intros h' orig. induction h'; auto.
-      simpl in *. destruct (o==o0). discriminate.
+  simpl. apply TypeCasesU.
+  - assert (forall h op,
+      find_op_case h op = None ->
+      find_op_case (Sub.h_shift h 1 i) op = None).
+    * intros h' op' orig. induction h'; auto.
+      simpl in *. destruct (op'==o). discriminate.
       apply IHh'. assumption.
-    * apply H2. assumption.
+    * apply H5. assumption.
   - apply IHh; assumption.
   - rewrite ctx_insert_extend. rewrite ctx_insert_extend.
-    assert (i+1+1=i+2) by omega. rewrite H2. apply IHc; assumption.
+    assert (i+1+1=i+2) by omega. rewrite H5. apply IHc; assumption.
 }
 Qed.
 
@@ -167,25 +181,32 @@ apply h_insert_typesafe. assumption.
 Qed.
 
 
-Fixpoint v_negshift_typesafe v (Γ:ctx) A i {struct v} :
-  has_vtype Γ v A -> v_no_var_j v i ->
+Fixpoint v_negshift_typesafe 
+  Γ v A (orig : has_vtype Γ v A) i {struct orig} :
+  v_no_var_j v i ->
   has_vtype (ctx_remove_var Γ i) (Sub.v_negshift v 1 i) A
 
-with c_negshift_typesafe c (Γ:ctx) C i {struct c} :
-  has_ctype Γ c C -> c_no_var_j c i ->
+with c_negshift_typesafe 
+  Γ c C (orig : has_ctype Γ c C) i {struct orig} :
+  c_no_var_j c i ->
   has_ctype (ctx_remove_var Γ i) (Sub.c_negshift c 1 i) C
 
-with h_negshift_typesafe h (Γ:ctx) Σ D i {struct h} :
-  has_htype Γ h Σ D -> h_no_var_j h i ->
+with h_negshift_typesafe 
+  Γ h Σ D (orig : has_htype Γ h Σ D) i {struct orig} :
+  h_no_var_j h i ->
   has_htype (ctx_remove_var Γ i) (Sub.h_negshift h 1 i) Σ D.
 Proof.
 {
-intros orig no_var. simpl in no_var. apply TypeV; inv orig.
+intros no_var. simpl in no_var. apply TypeV; inv orig.
 { apply ctx_remove_wf. assumption. }
 { assumption. }
-destruct v.
+destruct H1.
 + clear v_negshift_typesafe c_negshift_typesafe h_negshift_typesafe.
-  simpl. destruct v as (name, num). simpl. inv H1.
+  simpl. apply TypeUnit.
++ clear v_negshift_typesafe c_negshift_typesafe h_negshift_typesafe.
+  simpl. apply TypeInt.
++ clear v_negshift_typesafe c_negshift_typesafe h_negshift_typesafe.
+  simpl.
   assert (
     (if i <=? num then (name, num - 1) else (name, num))
       = (name, if i <=? num then num - 1 else num) ) 
@@ -193,264 +214,272 @@ destruct v.
   rewrite same. destruct (i <=? num) eqn:cmp.
   - apply TypeVar. rewrite <-get_ctx_remove_changed; apply leb_complete in cmp.
     * destruct num. destruct no_var. omega.
-      simpl. assert (num-0=num) by omega. rewrite H1. assumption.
+      simpl. assert (num-0=num) by omega. rewrite H2. assumption.
     * destruct cmp.
       ++ destruct no_var. reflexivity.
       ++ omega.
   - apply TypeVar. rewrite <-get_ctx_remove_unchanged.
     assumption. apply leb_iff_conv in cmp. assumption.
-+ clear v_negshift_typesafe c_negshift_typesafe h_negshift_typesafe.
-  simpl. inv H1. apply TypeUnit.
-+ clear v_negshift_typesafe c_negshift_typesafe h_negshift_typesafe.
-  simpl. inv H1. apply TypeInt.
-+ specialize (v_negshift_typesafe v) as IHv.
++ specialize (v_negshift_typesafe _ _ _ H1) as IHv1.
+  specialize (v_negshift_typesafe _ _ _ H2) as IHv2.
   clear v_negshift_typesafe c_negshift_typesafe h_negshift_typesafe.
-  simpl. inv H1. apply TypeInl. apply IHv.
-  assumption. assumption.
-+ specialize (v_negshift_typesafe v) as IHv.
-  clear v_negshift_typesafe c_negshift_typesafe h_negshift_typesafe.
-  simpl. inv H1. apply TypeInr. apply IHv.
-  assumption. assumption.
-+ specialize (v_negshift_typesafe v1) as IHv1.
-  specialize (v_negshift_typesafe v2) as IHv2.
-  clear v_negshift_typesafe c_negshift_typesafe h_negshift_typesafe.
-  simpl. inv H1. destruct no_var. apply TypePair. 
+  simpl. destruct no_var. apply TypePair. 
   apply IHv1; assumption. apply IHv2; assumption.
-+ specialize (c_negshift_typesafe c) as IHc.
++ specialize (v_negshift_typesafe _ _ _ H1) as IHv.
   clear v_negshift_typesafe c_negshift_typesafe h_negshift_typesafe.
-  simpl. inv H1. apply TypeFun. rewrite ctx_remove_extend.
+  simpl. apply TypeInl. apply IHv. assumption.
++ specialize (v_negshift_typesafe _ _ _ H1) as IHv.
+  clear v_negshift_typesafe c_negshift_typesafe h_negshift_typesafe.
+  simpl. apply TypeInr. apply IHv. assumption.
++ specialize (c_negshift_typesafe _ _ _ H1) as IHc.
+  clear v_negshift_typesafe c_negshift_typesafe h_negshift_typesafe.
+  simpl. apply TypeFun. rewrite ctx_remove_extend.
   apply IHc; assumption.
-+ specialize (h_negshift_typesafe h) as IHh.
-  specialize (c_negshift_typesafe c) as IHc.
++ specialize (h_negshift_typesafe _ _ _ _ H2) as IHh.
+  specialize (c_negshift_typesafe _ _ _ H1) as IHc.
   clear v_negshift_typesafe c_negshift_typesafe h_negshift_typesafe.
-  simpl. inv H1. destruct no_var.
+  simpl. destruct no_var.
   apply TypeHandler. rewrite ctx_remove_extend.
   apply IHc; assumption. apply IHh; assumption.
++ specialize (v_negshift_typesafe _ _ _ H1) as IHv.
+  clear v_negshift_typesafe c_negshift_typesafe h_negshift_typesafe.
+  eapply TypeVSubtype.
+  - apply IHv. assumption.
+  - assumption.
 }{
-intros orig no_var. simpl in no_var. apply TypeC; inv orig.
+intros no_var. simpl in no_var. apply TypeC; inv orig.
 { apply ctx_remove_wf. assumption. }
 { assumption. }
-destruct c.
-+ specialize (v_negshift_typesafe v) as IHv.
+destruct H1.
++ specialize (v_negshift_typesafe _ _ _ H1) as IHv.
   clear v_negshift_typesafe c_negshift_typesafe h_negshift_typesafe.
-  simpl. inv H1. apply TypeRet. apply IHv; assumption.
-+ specialize (v_negshift_typesafe v) as IHv.
-  specialize (c_negshift_typesafe c) as IHc.
+  simpl. apply TypeRet. apply IHv; assumption.
++ specialize (v_negshift_typesafe _ _ _ H1) as IHv.
+  specialize (c_negshift_typesafe _ _ _ H2) as IHc.
   clear v_negshift_typesafe c_negshift_typesafe h_negshift_typesafe.
-  simpl. inv H1. destruct no_var. eapply TypeΠMatch.
-  - apply IHv. exact H7. assumption.
+  simpl. destruct no_var. eapply TypeΠMatch.
+  - apply IHv. assumption.
   - rewrite ctx_remove_extend. rewrite ctx_remove_extend.
     assert (i+1+1=i+2) as SSi by omega. rewrite SSi. apply IHc; assumption.
-+ specialize (v_negshift_typesafe v) as IHv.
-  specialize (c_negshift_typesafe c1) as IHc1.
-  specialize (c_negshift_typesafe c2) as IHc2.
++ specialize (v_negshift_typesafe _ _ _ H1) as IHv.
+  specialize (c_negshift_typesafe _ _ _ H2) as IHc1.
+  specialize (c_negshift_typesafe _ _ _ H3) as IHc2.
   clear v_negshift_typesafe c_negshift_typesafe h_negshift_typesafe.
-  simpl. inv H1. destruct no_var. destruct H0. destruct H2.
+  simpl. destruct no_var. destruct H5.
   eapply TypeΣMatch.
-  - apply IHv. exact H9. assumption.
+  - apply IHv. assumption.
   - rewrite ctx_remove_extend. apply IHc1; assumption. 
-  - rewrite ctx_remove_extend. apply IHc2; assumption. 
-+ specialize (v_negshift_typesafe v) as IHv.
-  specialize (v_negshift_typesafe v0) as IHv0.
+  - rewrite ctx_remove_extend. apply IHc2; assumption.
++ specialize (c_negshift_typesafe _ _ _ H1) as IHc1.
+  specialize (c_negshift_typesafe _ _ _ H2) as IHc2.
   clear v_negshift_typesafe c_negshift_typesafe h_negshift_typesafe.
-  simpl. inv H1. destruct no_var. eapply TypeApp.
-  - apply IHv. exact H5. assumption.
+  simpl. destruct no_var. eapply TypeDoBind.
+  - apply IHc1. assumption.
+  - rewrite ctx_remove_extend. apply IHc2; assumption.
++ specialize (v_negshift_typesafe _ _ _ H1) as IHv.
+  specialize (v_negshift_typesafe _ _ _ H2) as IHv0.
+  clear v_negshift_typesafe c_negshift_typesafe h_negshift_typesafe.
+  simpl. destruct no_var. eapply TypeApp.
+  - apply IHv. assumption.
   - apply IHv0; assumption.
-+ specialize (v_negshift_typesafe v) as IHv.
-  specialize (c_negshift_typesafe c) as IHc.
++ specialize (v_negshift_typesafe _ _ _ H1) as IHv.
+  specialize (c_negshift_typesafe _ _ _ H2) as IHc.
   clear v_negshift_typesafe c_negshift_typesafe h_negshift_typesafe.
-  simpl. inv H1. destruct no_var. eapply TypeOp. exact H8.
-  - apply IHv; assumption.
-  - rewrite ctx_remove_extend. apply IHc; assumption.
-+ specialize (c_negshift_typesafe c1) as IHc1.
-  specialize (c_negshift_typesafe c2) as IHc2.
+  simpl. destruct no_var. eapply TypeHandle.
+  - apply IHv. assumption.
+  - apply IHc; assumption.
++ specialize (c_negshift_typesafe _ _ _ H1) as IHc1.
+  specialize (c_negshift_typesafe _ _ _ H2) as IHc2.
   clear v_negshift_typesafe c_negshift_typesafe h_negshift_typesafe.
-  simpl. inv H1. destruct no_var. eapply TypeLetRec.
+  simpl. destruct no_var. eapply TypeLetRec.
   - rewrite ctx_remove_extend. rewrite ctx_remove_extend.
     assert (i+1+1=i+2) as SSi by omega. rewrite SSi.
-    apply IHc1. exact H8. assumption.
+    apply IHc1. assumption.
   - rewrite ctx_remove_extend.  apply IHc2; assumption.
-+ specialize (c_negshift_typesafe c1) as IHc1.
-  specialize (c_negshift_typesafe c2) as IHc2.
++ specialize (v_negshift_typesafe _ _ _ H2) as IHv.
+  specialize (c_negshift_typesafe _ _ _ H3) as IHc.
   clear v_negshift_typesafe c_negshift_typesafe h_negshift_typesafe.
-  simpl. inv H1. destruct no_var. eapply TypeDoBind.
-  - apply IHc1. exact H7. assumption.
-  - rewrite ctx_remove_extend. apply IHc2; assumption.
-+ specialize (v_negshift_typesafe v) as IHv.
-  specialize (c_negshift_typesafe c) as IHc.
+  simpl. destruct no_var. eapply TypeOp. exact H1.
+  - apply IHv; assumption.
+  - rewrite ctx_remove_extend. apply IHc; assumption.
++ specialize (c_negshift_typesafe _ _ _ H1) as IHc.
   clear v_negshift_typesafe c_negshift_typesafe h_negshift_typesafe.
-  simpl. inv H1. destruct no_var. eapply TypeHandle.
-  - apply IHv. exact H5. assumption.
-  - apply IHc; assumption.
+  eapply TypeCSubtype.
+  - apply IHc. assumption.
+  - assumption.
 }{
-intros orig no_var; simpl; apply TypeH; inv orig.
-{ apply ctx_remove_wf. assumption. }
-assumption. assumption.
-destruct h.
-+ clear v_negshift_typesafe c_negshift_typesafe h_negshift_typesafe.
-  simpl. inv H2. apply TypeCasesØ.
-+ specialize (h_negshift_typesafe h) as IHh.
-  specialize (c_negshift_typesafe c) as IHc.
+intros no_var; simpl; apply TypeH; inv orig.
+apply ctx_remove_wf. assumption. assumption. assumption.
+destruct H2.
++ simpl. clear v_negshift_typesafe c_negshift_typesafe h_negshift_typesafe.
+  apply TypeCasesØ.
++ specialize (h_negshift_typesafe _ _ _ _ H3) as IHh.
+  specialize (c_negshift_typesafe _ _ _ H4) as IHc.
   clear v_negshift_typesafe c_negshift_typesafe h_negshift_typesafe.
-  simpl in no_var. destruct no_var. simpl. inv H2. apply TypeCasesU.
-  - assert (forall h,
-      find_op_case h o = None ->
-      find_op_case (Sub.h_negshift h 1 i) o = None) as no_find.
-    * intros h' orig. induction h'; auto.
-      simpl in *. destruct (o==o0). discriminate.
-      apply IHh'; assumption.
-    * apply no_find. assumption.
-  - apply IHh; assumption. 
+  simpl. apply TypeCasesU.
+  - assert (forall h op,
+      find_op_case h op = None ->
+      find_op_case (Sub.h_negshift h 1 i) op = None).
+    * intros h' op' orig. induction h'; auto.
+      simpl in *. destruct (op'==o). discriminate.
+      apply IHh'. assumption.
+    * apply H5. assumption.
+  - apply IHh. destruct no_var. assumption.
   - rewrite ctx_remove_extend. rewrite ctx_remove_extend.
-    assert (i+1+1=i+2) as SSi by omega. rewrite SSi. apply IHc; assumption.
+    assert (i+1+1=i+2) by omega. rewrite H5.
+    apply IHc. destruct no_var. assumption.
 }
 Qed.
 
-
-Fixpoint v_subs_typesafe v Γ A i v_s A_s {struct v}:
-  has_vtype Γ v A -> get_vtype Γ i = Some A_s ->
-  has_vtype Γ v_s A_s ->
+Fixpoint v_subs_typesafe 
+  Γ v A (orig: has_vtype Γ v A) i v_s A_s {struct orig}:
+  get_vtype Γ i = Some A_s -> has_vtype Γ v_s A_s ->
   has_vtype Γ (Sub.v_sub v (i, v_s)) A
-with c_subs_typesafe c Γ C i v_s A_s {struct c}:
-  has_ctype Γ c C -> get_vtype Γ i = Some A_s ->
-  has_vtype Γ v_s A_s ->
+with c_subs_typesafe
+  Γ c C (orig: has_ctype Γ c C) i v_s A_s {struct orig}:
+  get_vtype Γ i = Some A_s -> has_vtype Γ v_s A_s ->
   has_ctype Γ (Sub.c_sub c (i, v_s)) C
-with h_subs_typesafe h Γ Σ D i v_s A_s {struct h}:
-  has_htype Γ h Σ D -> get_vtype Γ i = Some A_s ->
-  has_vtype Γ v_s A_s ->
+with h_subs_typesafe
+  Γ h Σ D (orig: has_htype Γ h Σ D) i v_s A_s {struct orig}:
+  get_vtype Γ i = Some A_s -> has_vtype Γ v_s A_s ->
   has_htype Γ (Sub.h_sub h (i, v_s)) Σ D.
 Proof.
 all: assert (forall i, i+1=S i) as Si by (intro; omega).
 all: assert (forall i, i+2=S(S i)) as SSi by (intro; omega).
 {
-intros orig gets vs_types. apply TypeV; inv orig.
-assumption. assumption. destruct v.
+intros gets vs_types. apply TypeV; inv orig.
+assumption. assumption. destruct H1.
 + clear v_subs_typesafe c_subs_typesafe h_subs_typesafe.
-  simpl. destruct v as (name, num). simpl. inv H1.
-  destruct (num =? i) eqn:cmp.
-  - apply Nat.eqb_eq in cmp. rewrite cmp in *. rewrite H6 in gets.
+  simpl. apply TypeUnit.
++ clear v_subs_typesafe c_subs_typesafe h_subs_typesafe.
+  simpl. apply TypeInt.
++ clear v_subs_typesafe c_subs_typesafe h_subs_typesafe.
+  simpl. destruct (num =? i) eqn:cmp.
+  - apply Nat.eqb_eq in cmp. rewrite cmp in *. rewrite H1 in gets.
     injection gets. intro. subst. inv vs_types. assumption.
   - apply TypeVar. assumption.
-+ clear v_subs_typesafe c_subs_typesafe h_subs_typesafe.
-  simpl. inv H1. apply TypeUnit.
-+ clear v_subs_typesafe c_subs_typesafe h_subs_typesafe.
-  simpl. inv H1. apply TypeInt.
-+ specialize (v_subs_typesafe v) as IHv.
++ specialize (v_subs_typesafe _ _ _ H1) as IHv1.
+  specialize (v_subs_typesafe _ _ _ H2) as IHv2.
   clear v_subs_typesafe c_subs_typesafe h_subs_typesafe.
-  simpl. inv H1. apply TypeInl. eapply IHv.
-  assumption. exact gets. assumption.
-+ specialize (v_subs_typesafe v) as IHv.
+  simpl. apply TypePair.
+  eapply IHv1. exact gets. assumption.
+  eapply IHv2. exact gets. assumption.
++ specialize (v_subs_typesafe _ _ _ H1) as IHv.
   clear v_subs_typesafe c_subs_typesafe h_subs_typesafe.
-  simpl. inv H1. apply TypeInr. eapply IHv.
-  assumption. exact gets. assumption.
-+ specialize (v_subs_typesafe v1) as IHv1.
-  specialize (v_subs_typesafe v2) as IHv2.
+  simpl. apply TypeInl. eapply IHv. exact gets. assumption.
++ specialize (v_subs_typesafe _ _ _ H1) as IHv.
   clear v_subs_typesafe c_subs_typesafe h_subs_typesafe.
-  simpl. inv H1. apply TypePair.
-  eapply IHv1. assumption. exact gets. assumption.
-  eapply IHv2. assumption. exact gets. assumption.
-+ specialize (c_subs_typesafe c) as IHc.
-  specialize (v_subs_typesafe v_s) as IHvs.
+  simpl. apply TypeInr. eapply IHv. exact gets. assumption.
++ specialize (c_subs_typesafe _ _ _ H1) as IHc.
+  specialize (v_subs_typesafe _ _ _ vs_types) as IHvs.
   clear v_subs_typesafe c_subs_typesafe h_subs_typesafe.
-  simpl. inv H1. apply TypeFun. eapply IHc.
-  assumption. rewrite Si. exact gets. apply v_shift_typesafe.
-  assumption. inv H0. assumption.
-+ specialize (h_subs_typesafe h) as IHh.
-  specialize (c_subs_typesafe c) as IHc.
+  simpl. apply TypeFun. eapply IHc.
+  rewrite Si. exact gets.
+  apply v_shift_typesafe. assumption. inv H0. assumption.
++ specialize (h_subs_typesafe _ _ _ _ H2) as IHh.
+  specialize (c_subs_typesafe _ _ _ H1) as IHc.
   clear v_subs_typesafe c_subs_typesafe h_subs_typesafe.
-  simpl. inv H1. apply TypeHandler.
-  - eapply IHc. assumption. rewrite Si. exact gets.
-    apply v_shift_typesafe. assumption. inv H0. inv H3. assumption.
-  - eapply IHh. assumption. exact gets. assumption.
+  simpl. apply TypeHandler.
+  - eapply IHc. rewrite Si. exact gets.
+    apply v_shift_typesafe. assumption. inv H0. inv H5. assumption.
+  - eapply IHh. exact gets. assumption.
++ specialize (v_subs_typesafe _ _ _ H1) as IHv.
+  clear v_subs_typesafe c_subs_typesafe h_subs_typesafe.
+  eapply TypeVSubtype.
+  - eapply IHv. exact gets. assumption.
+  - assumption. 
 }{
-intros orig gets vs_types. apply TypeC; inv orig.
-assumption. assumption. destruct c.
-+ specialize (v_subs_typesafe v) as IHv.
+intros gets vs_types. apply TypeC; inv orig.
+assumption. assumption. destruct H1.
++ specialize (v_subs_typesafe _ _ _ H1) as IHv.
   clear v_subs_typesafe c_subs_typesafe h_subs_typesafe.
-  simpl. inv H1. apply TypeRet. eapply IHv.
-  assumption. exact gets. assumption.
-+ specialize (v_subs_typesafe v) as IHv.
-  specialize (c_subs_typesafe c) as IHc.
+  simpl. apply TypeRet. eapply IHv. exact gets. assumption.
++ specialize (v_subs_typesafe _ _ _ H1) as IHv.
+  specialize (c_subs_typesafe _ _ _ H2) as IHc.
   clear v_subs_typesafe c_subs_typesafe h_subs_typesafe.
-  simpl. inv H1. eapply TypeΠMatch.
-  - eapply IHv. exact H7. exact gets. assumption.
-  - eapply IHc. assumption. rewrite SSi. exact gets. 
+  simpl. eapply TypeΠMatch.
+  - eapply IHv. exact gets. assumption.
+  - eapply IHc. rewrite SSi. exact gets. 
     rewrite <-(v_shift_shift 1 1 0).
     apply v_shift_typesafe. apply v_shift_typesafe. assumption.
-    all: inv H7; inv H2; assumption.
-+ specialize (v_subs_typesafe v) as IHv.
-  specialize (c_subs_typesafe c1) as IHc1.
-  specialize (c_subs_typesafe c2) as IHc2.
+    all: inv H1; inv H4; assumption.
++ specialize (v_subs_typesafe _ _ _ H1) as IHv.
+  specialize (c_subs_typesafe _ _ _ H2) as IHc1.
+  specialize (c_subs_typesafe _ _ _ H3) as IHc2.
   clear v_subs_typesafe c_subs_typesafe h_subs_typesafe.
-  simpl. inv H1. eapply TypeΣMatch.
-  - eapply IHv. exact H9. exact gets. assumption.
-  - eapply IHc1. assumption. rewrite Si. exact gets.
+  simpl. eapply TypeΣMatch.
+  - eapply IHv. exact gets. assumption.
+  - eapply IHc1. rewrite Si. exact gets.
     apply v_shift_typesafe. assumption.
-    inv H9. inv H2. assumption. 
-  - eapply IHc2. assumption. rewrite Si. exact gets.
+    inv H1. inv H5. assumption. 
+  - eapply IHc2. rewrite Si. exact gets.
     apply v_shift_typesafe. assumption.
-    inv H9. inv H2. assumption. 
-+ specialize (v_subs_typesafe v) as IHv.
-  specialize (v_subs_typesafe v0) as IHv0.
+    inv H1. inv H5. assumption. 
++ specialize (c_subs_typesafe _ _ _ H1) as IHc1.
+  specialize (c_subs_typesafe _ _ _ H2) as IHc2.
   clear v_subs_typesafe c_subs_typesafe h_subs_typesafe.
-  simpl. inv H1. eapply TypeApp.
-  - eapply IHv. exact H5. exact gets. assumption.
-  - eapply IHv0. assumption. exact gets. assumption.
-+ specialize (v_subs_typesafe v) as IHv.
-  specialize (c_subs_typesafe c) as IHc.
-  clear v_subs_typesafe c_subs_typesafe h_subs_typesafe.
-  simpl. inv H1. eapply TypeOp. exact H8.
-  - eapply IHv. assumption. exact gets. assumption.
-  - eapply IHc. assumption. rewrite Si. exact gets. 
+  simpl. eapply TypeDoBind.
+  - eapply IHc1. exact gets. assumption.
+  - eapply IHc2. rewrite Si. exact gets.
     apply v_shift_typesafe. assumption.
-    inv H10. inv H1. assumption.
-+ specialize (c_subs_typesafe c1) as IHc1.
-  specialize (c_subs_typesafe c2) as IHc2.
+    inv H1. inv H4. assumption.
++ specialize (v_subs_typesafe _ _ _ H1) as IHv.
+  specialize (v_subs_typesafe _ _ _ H2) as IHv0.
   clear v_subs_typesafe c_subs_typesafe h_subs_typesafe.
-  simpl. inv H1. eapply TypeLetRec.
-  - rewrite SSi. eapply IHc1. exact H8. exact gets.
+  simpl. eapply TypeApp.
+  - eapply IHv. exact gets. assumption.
+  - eapply IHv0. exact gets. assumption.
++ specialize (v_subs_typesafe _ _ _ H1) as IHv.
+  specialize (c_subs_typesafe _ _ _ H2) as IHc.
+  clear v_subs_typesafe c_subs_typesafe h_subs_typesafe.
+  simpl. eapply TypeHandle.
+  - eapply IHv. exact gets. assumption.
+  - eapply IHc. exact gets. assumption.
++ specialize (c_subs_typesafe _ _ _ H1) as IHc1.
+  specialize (c_subs_typesafe _ _ _ H2) as IHc2.
+  clear v_subs_typesafe c_subs_typesafe h_subs_typesafe.
+  simpl. eapply TypeLetRec.
+  - rewrite SSi. eapply IHc1. exact gets.
     rewrite <-(v_shift_shift 1 1 0).
     apply v_shift_typesafe. apply v_shift_typesafe. assumption.
-    all: inv H8; inv H1. 2: assumption. inv H6. assumption. 
-  - eapply IHc2. assumption. rewrite Si. exact gets.
+    all: inv H1; inv H3. 2: assumption. inv H7. assumption. 
+  - eapply IHc2. rewrite Si. exact gets.
     apply v_shift_typesafe. assumption.
-    inv H9. inv H1. assumption.
-+ specialize (c_subs_typesafe c1) as IHc1.
-  specialize (c_subs_typesafe c2) as IHc2.
+    inv H1. inv H3. assumption.
++ specialize (v_subs_typesafe _ _ _ H2) as IHv.
+  specialize (c_subs_typesafe _ _ _ H3) as IHc.
   clear v_subs_typesafe c_subs_typesafe h_subs_typesafe.
-  simpl. inv H1. eapply TypeDoBind.
-  - eapply IHc1. exact H7. exact gets. assumption.
-  - eapply IHc2. assumption. rewrite Si. exact gets.
+  simpl. eapply TypeOp. exact H1.
+  - eapply IHv. exact gets. assumption.
+  - eapply IHc. rewrite Si. exact gets. 
     apply v_shift_typesafe. assumption.
-    inv H7. inv H2. assumption.
-+ specialize (v_subs_typesafe v) as IHv.
-  specialize (c_subs_typesafe c) as IHc.
+    inv H3. inv H4. assumption.
++ specialize (c_subs_typesafe _ _ _ H1) as IHc.
   clear v_subs_typesafe c_subs_typesafe h_subs_typesafe.
-  simpl. inv H1. eapply TypeHandle.
-  - eapply IHv. exact H5. exact gets. assumption.
-  - eapply IHc. assumption. exact gets. assumption.
+  eapply TypeCSubtype.
+  - eapply IHc. exact gets. assumption.
+  - assumption.
 }{
-intros orig gets vs_types; simpl; apply TypeH; inv orig.
+intros gets vs_types; simpl; apply TypeH; inv orig.
 assumption. assumption. assumption.
-destruct h.
-+ clear v_subs_typesafe c_subs_typesafe h_subs_typesafe.
-  inv H2. apply TypeCasesØ.
-+ specialize (h_subs_typesafe h) as IHh.
-  specialize (c_subs_typesafe c) as IHc.
+destruct H2.
++ clear v_subs_typesafe c_subs_typesafe h_subs_typesafe. apply TypeCasesØ.
++ specialize (h_subs_typesafe _ _ _ _ H3) as IHh.
+  specialize (c_subs_typesafe _ _ _ H4) as IHc.
   clear v_subs_typesafe c_subs_typesafe h_subs_typesafe.
-  simpl. inv H2. apply TypeCasesU.
-  - assert (forall h,
+  simpl. apply TypeCasesU.
+  - assert (forall h o,
       find_op_case h o = None ->
       find_op_case (Sub.h_sub h (i, v_s)) o = None) as no_find.
-    * intros h' orig. induction h'; auto.
+    * intros h' o orig. induction h'; auto.
       simpl in *. destruct (o==o0). discriminate.
       apply IHh'. assumption.
     * apply no_find. assumption.
-  - eapply IHh. exact H12. exact gets. assumption.
-  - rewrite SSi. eapply IHc. assumption. exact gets.
+  - eapply IHh. exact gets. assumption.
+  - rewrite SSi. eapply IHc. exact gets.
     rewrite <-(v_shift_shift 1 1 0).
     apply v_shift_typesafe. apply v_shift_typesafe. assumption.
-    all: inv H0. 2: assumption. inv H12. apply WfFun; assumption.
+    all: inv H0. 2: assumption. apply WfFun; assumption.
 }
 Qed.
 
